almost complete rel_kernel_to_program lemma

src/rel_hoare.lean
@@ -18,15 +18,15 @@ def rel_hoare_memory (P : memory τ → memory τ → Prop) (k₁ : kernel σ τ
 
 namespace rel_hoare
 
-lemma seq {P Q R} {k₁ k₁' k₂ k₂' : kernel σ τ} : {* P *} k₁ ~ k₁' {* Q *} → {* Q *} k₂ ~ k₂' {* R *} → {* P *} (k₁ ;; k₂) ~ (k₁' ;; k₂') {* R *} := begin
-    intros h₁ h₂ n s u ac m m' o o' hp hseq₁ hseq₂,
-    cases hseq₁,
-    cases hseq₂,
-    cases hseq₁_hk,
-    cases hseq₂_hk,
-    unfold rel_hoare at h₁ h₂,
-    apply h₂ n _ _ _ _ _ _ _ _ _ hseq₁_hk_a_1 hseq₂_hk_a_1,
-end
+-- lemma seq {P Q R} {k₁ k₁' k₂ k₂' : kernel σ τ} : {* P *} k₁ ~ k₁' {* Q *} → {* Q *} k₂ ~ k₂' {* R *} → {* P *} (k₁ ;; k₂) ~ (k₁' ;; k₂') {* R *} := begin
+--     intros h₁ h₂ n s u ac m m' o o' hp hseq₁ hseq₂,
+--     cases hseq₁,
+--     cases hseq₂,
+--     cases hseq₁_hk,
+--     cases hseq₂_hk,
+--     unfold rel_hoare at h₁ h₂,
+--     apply h₂ n _ _ _ _ _ _ _ _ _ hseq₁_hk_a_1 hseq₂_hk_a_1,
+-- end
 
 end rel_hoare
 
@@ -35,24 +35,87 @@ def rel_hoare_program (init₁ : ℕ → σ₁) (init₂ : ℕ → σ₂) (P : m
 
 -- notation `{* ` P : 1 ` *} ` p₁ : 1 ` ~ ` p₂ : 1 ` {* ` Q : 1 ` *}` := rel_hoare_state P p₁ p₂ Q
 
-def rel_kernel_to_program (k₁ : kernel σ₁ τ₁) (k₂ : kernel σ₂ τ₂) (init₁ : ℕ → σ₁) (init₂ : ℕ → σ₂) (P Q : memory τ₁ → memory τ₂ → Prop) (f₁ : memory τ₁ → ℕ) (f₂ : memory τ₂ → ℕ)
+lemma rel_kernel_to_program (k₁ : kernel σ₁ τ₁) (k₂ : kernel σ₂ τ₂) (init₁ : ℕ → σ₁) (init₂ : ℕ → σ₂) (P Q : memory τ₁ → memory τ₂ → Prop) (f₁ : memory τ₁ → ℕ) (f₂ : memory τ₂ → ℕ)
  (h : {* λ n₁ s₁ ac₁ n₂ s₂ ac₂, ∃ m₁ m₂, s₁.syncable m₁ ∧ s₂.syncable m₂ ∧ n₁ = f₁ m₁ ∧ n₂ = f₂ m₂ ∧
  (∀ i : fin n₁, (s₁.threads.nth i).tlocal = init₁ i) ∧ (∀ i : fin n₂, (s₂.threads.nth i).tlocal = init₂ i) *} k₁ ~ k₂ 
- {* λ n₁ s₁ ac₁ n₂ s₂ ac₂, ∃ m₁ m₂, s₁.syncable m₁ ∧ s₂.syncable m₂ ∧ Q m₁ m₂ *} ) : 
+ {* λ n₁ s₁ ac₁ n₂ s₂ ac₂, ∃ m₁ m₂, s₁.syncable m₁ ∧ s₂.syncable m₂ ∧ Q m₁ m₂ *} ) : -- if I have to proof syncability of s₁, do I really have to assume termination of the left?
  rel_hoare_program init₁ init₂ P (program.intro f₁ k₁) (program.intro f₂ k₂) Q :=
 begin
     unfold rel_hoare_state at h,
     unfold rel_hoare_program,
     intros m₁ m₁' m₂ hp hep,
     cases hep,
-    cases hep_h,
-    specialize h (f₁ m₁) (f₂ m₂),
-    apply exists.intro,
+    specialize h (f₁ m₁) (f₂ m₂) 
+        (init_state init₁ f₁ m₁)
+        hep_s'
+        (init_state init₂ f₂ m₂)
+        (vector.repeat tt (f₁ m₁))
+        (vector.repeat tt (f₂ m₂)),
+    have hh : (∃ (s₂' : state (f₂ m₂) σ₂ τ₂), exec_state k₂ (vector.repeat tt (f₂ m₂)) (init_state init₂ f₂ m₂) s₂' ∧
+    ∃ (m₁_1 : memory τ₁) (m₂_1 : memory τ₂), state.syncable hep_s' m₁_1 ∧ state.syncable s₂' m₂_1 ∧ Q m₁_1 m₂_1) := begin
+        apply h,
+        {
+            apply exists.intro m₁,
+            apply exists.intro m₂,
+            apply and.intro,
+            {
+                apply init_state_syncable,
+            }, {
+                apply and.intro,
+                {
+                    apply init_state_syncable,
+                },
+                {
+                    apply and.intro,
+                    {
+                        refl,
+                    },
+                    {
+                        apply and.intro,
+                        {
+                            refl,
+                        },
+                        {
+                            apply and.intro,
+                            {
+                                simp,
+                                intro i,
+                                rw vector.range_nth,
+                            },
+                            {
+                                simp,
+                                intro i,
+                                rw vector.range_nth,
+                            }
+                        }
+                    }
+                }
+            }
+        }, {
+            exact hep_he,
+        }
+    end,
+    cases hh,
+    cases hh_h,
+    cases hh_h_right with m₁'',
+    cases hh_h_right_h with m₂',
+    apply exists.intro m₂',
     apply and.intro,
     {
-        apply exec_prog.intro,
-        apply exec_memory.intro,
-
+        apply exec_prog.intro _ _ _ _ _ hh_w,
+        { exact hh_h_right_h_h.right.left, },
+        { exact hh_h_left, },
+    }, {
+        have hu : m₁' = m₁'' := begin
+            by_cases hz : 0 < (f₁ m₁),
+            {
+                apply state.syncable_unique hep_hsync hh_h_right_h_h.left hz,
+            }, {
+                sorry
+            }
+        end,
+        subst hu,
+        exact hh_h_right_h_h.right.right,
     }
 end
 
